Evaluator.v
@@ -19,8 +19,6 @@ Fixpoint isNat (t : tree) : bool :=
 end.
 Fixpoint isValue (t: tree) : bool :=
   match t with
-    (*| lvar _ _ => true
-    | fvar _ _ => true *)
     | uu => true
     | ttrue => true
     | tfalse => true
@@ -31,6 +29,7 @@ Fixpoint isValue (t: tree) : bool :=
     | succ e1 => (isValue e1)
     | notype_lambda _ => true
     | _ => false end.
+
 Definition getPair t : {t': option (tree*tree) | forall t1 t2, t' = Some (t1, t2) <-> t = pp t1 t2}.
   Proof.
     exists ( match t with
@@ -45,7 +44,7 @@ Definition getPair t : {t': option (tree*tree) | forall t1 t2, t' = Some (t1, t2
        | notype_lambda body => Some body
        | _ => None end).
     destruct t; steps.
-  Defined.  
+  Defined.
 
   Definition getLR t : {t': option tree | forall t1, t' = Some t1 <-> (t = tleft t1 \/ t = tright t1)}.
   Proof.
@@ -54,10 +53,10 @@ Definition getPair t : {t': option (tree*tree) | forall t1 t2, t' = Some (t1, t2
        | tright t' => Some t'
        | _ => None end).
     destruct t; steps.
-  Defined.    
+  Defined.
 
 
-(* Evaluator *)
+(* Evaluator (smallstep) *)
 Fixpoint ss_eval (t: tree) {struct t}: (option tree) :=
   match t with
     | ite ttrue t1 t2 => Some t1
@@ -81,20 +80,20 @@ Fixpoint ss_eval (t: tree) {struct t}: (option tree) :=
                 if (isValue e1) && (isValue e2)
                 then Some e2
                 else option_map pi2 (ss_eval t) end
-                                                                                                       
+
     | app t1 t2 => match (isValue t1) with
                     | true => match getApp t1 with
-                             | exist _ None _ => option_map (app t1) (ss_eval t2) 
+                             | exist _ None _ => option_map (app t1) (ss_eval t2)
                              | exist _ (Some ts) _ =>
                                if (isValue t2)
                                then Some (open 0 ts t2)
                                else option_map (app t1) (ss_eval t2) end
                     | false => option_map (fun e => app e t2) (ss_eval t1) end
-                    
+
     | notype_tfix ts => Some (open 0 (open 1 ts zero) (notype_tfix ts))
 
     | succ t => option_map succ (ss_eval t)
-                          
+
     | tmatch t1 t0 ts => match t1 with
                        | zero => Some t0
                        | succ t2 =>
@@ -108,7 +107,7 @@ Fixpoint ss_eval (t: tree) {struct t}: (option tree) :=
                                    | tright v => Some (open 0 tr v)
                                    | _ => None end
                           else option_map (fun e => sum_match e tl tr) (ss_eval t)
-                            
+
     | tleft t => option_map tleft (ss_eval t)
     | tright t => option_map tright (ss_eval t)
 
@@ -122,6 +121,7 @@ Fixpoint ss_eval (t: tree) {struct t}: (option tree) :=
     | _ => None
   end.
 
+(* Compute a certain number of small steps *)
 Fixpoint ss_eval_n (t : tree) (k: nat) : (option tree) :=
   match k with
     | 0 => Some t
@@ -130,63 +130,12 @@ Fixpoint ss_eval_n (t : tree) (k: nat) : (option tree) :=
                | None => Some t end
   end.
 
+(* Entry point for evaluation *)
 Definition eval (t: tree) (k: nat): (option tree) :=
   ss_eval_n (erase_term t) k.
 
 
 (* Tactics *)
-Hint Rewrite Bool.andb_true_iff: bools.
-Hint Rewrite Bool.andb_false_iff: bools.
-Hint Rewrite Bool.orb_true_iff: bools.
-Hint Rewrite Bool.orb_false_iff: bools.
-Hint Rewrite Bool.negb_true_iff: bools.
-Hint Rewrite Bool.negb_false_iff: bools.
-Ltac bools :=
-  autorewrite with bools in *.
-       
-Ltac options :=
-unfold option_map in *.
-
-Ltac invert_constructor_equalities :=
-match goal with
-| H: ?F _ = ?F _ |- _ => is_constructor F; inversion H; clear H
-| H: ?F _ _ = ?F _ _ |- _ => is_constructor F; inversion H; clear H
-| H: ?F _ _ _ = ?F _ _ _ |- _ => is_constructor F; inversion H; clear H
-| H: ?F _ _ _ _ = ?F _ _ _ _ |- _ => is_constructor F; inversion H; clear H
-| H: ?F _ _ _ _ _ = ?F _ _ _ _ _ |- _ => is_constructor F; inversion H; clear H
-| H: ?F _ _ _ _ _ _ = ?F _ _ _ _ _ _ |- _ => is_constructor F; inversion H; clear H
-end. 
-
-Ltac custom_light :=
-  (intros) ||
-  (subst).
-
-Ltac destruct_match :=
-match goal with
-| [ |- context[match ?t with _ => _ end]] =>
-let matched := fresh "matched" in
-destruct t eqn:matched
-| [ H: context[match ?t with _ => _ end] |- _ ] =>
-let matched := fresh "matched" in
-destruct t eqn:matched
-end. 
-
-
-
-Ltac instantiate_eq_refl :=
-match goal with
-| H: _ |- _ => pose proof (proj1 (H _) eq_refl); clear H
-| H: _ |- _ => pose proof (proj2 (H _) eq_refl); clear H
-| H: _ |- _ => pose proof (H _ eq_refl); clear H
-| H: _ |- _ => pose proof (H _ _ eq_refl ); clear H
-| H: _ |- _ => pose proof (proj1 (H _ _ ) eq_refl); clear H
-| H: _ |- _ => pose proof (proj2 (H _ _ ) eq_refl); clear H
-| H: _ |- _ => pose proof (H _ _ _ eq_refl); clear H
-| H: _ |- _ => pose proof (H _ _ _ _ eq_refl); clear H
-| H: _ |- _ => pose proof (H _ _ _ _ _ eq_refl); clear H
-| H: _ |- _ => pose proof (H _ _ _ _ _ _ eq_refl); clear H
-end.
-                                               
 Ltac destruct_sig :=
 match goal with
   | H: _ |- context[let _ := getPair ?t in _ ]  => let fresh := fresh "getPair" in destruct (getPair t) (* eqn:fresh *)
@@ -195,6 +144,7 @@ match goal with
   | H: context[getApp ?t = _ ] |- _ => let fresh := fresh "getApp" in destruct (getApp t) (* eqn:fresh *)
   | H: context[_ = getApp ?t ] |- _ => let fresh := fresh "getApp" in destruct (getApp t) (* eqn:fresh *)
 end. (* match on type of t = sig *)
+
 Ltac destruct_ss_eval :=
   match goal with
     | H: context[ss_eval ?t] |- _ => destruct (ss_eval t) end.
@@ -219,14 +169,18 @@ Ltac ss_eval_step :=
 
 
 Lemma ss_eval_correct2: forall t t',(pfv t term_var = nil) -> scbv_step t t' ->  ss_eval t = Some t'.
-  intros.
-  induction H0 ;
-    repeat light || options || invert_constructor_equalities || ss_eval_step || destruct_sig || instantiate_eq_refl || list_utils || bools || rewrite <- isValueCorrect in * ||  eauto using fv_nil_top_level_var with smallstep values || destruct_match.
+  intros. induction H0 ; repeat light || options || invert_constructor_equalities || ss_eval_step || destruct_sig || instantiate_eq_refl || list_utils || bools || rewrite <- isValueCorrect in * ||  eauto using fv_nil_top_level_var with smallstep values || destruct_match.
 Qed.
 
 Lemma ss_eval_correct1: forall t t', ss_eval t = Some t' -> (pfv t term_var = nil) -> scbv_step t t'.
 Proof.
   induction t; intros ; repeat light ; destruct_ss_eval ; repeat light || options || bools || list_utils || instantiate_eq_refl || invert_constructor_equalities || rewrite isValueCorrect in * || destruct_sig || congruence ||  step_inversion cbv_value || destruct_match ; eauto using ss_eval_step, fv_nil_top_level_var with smallstep values . Qed.
+
+(* Main theorem : the evaluator corresponds to the small call-by-value steps *)
+Theorem ss_eval_correct : forall t t', (pfv t term_var = nil) -> (ss_eval t = Some t' <-> scbv_step t t').
+Proof.
+  intros. split ; eauto using ss_eval_correct1, ss_eval_correct2.
+Qed.
 
 
 (* Extraction *)
@@ -236,5 +190,4 @@ Extraction Language Ocaml.
 Set Extraction AccessOpaque.
 
 
-Extraction "evaluator.ml" eval. 
-    
+Extraction "evaluator.ml" eval.
