examples/natmatch.v
@@ -4,7 +4,7 @@ Require Extraction.
 Import Notations.UnTyped.
 
 
-Definition natmatch_example := Eval compute in 
+Definition natmatch_example := Eval compute in
   [|
    let pred :=
        def_rec ack m =>
@@ -13,13 +13,15 @@ Definition natmatch_example := Eval compute in
        | s m' => m'
        end
    in
-   pred 9      
+   pred 9
     |].
 
 
-Eval compute in eval natmatch_example 1000.
+Example natmatch : (eval natmatch_example 1000) =  Some [| 8 |].
+Proof.
+  native_compute; reflexivity. Qed.
 
-
+(* Extraction *)
 Extraction Language Ocaml.
 Set Extraction AccessOpaque.
-Extraction "natmatch.ml" natmatch_example eval. 
+Extraction "natmatch.ml" natmatch_example eval.
